SkipList/FStar/SkipListHashes.fst
@@ -1,0 +1,24 @@
+module SkipListHashes
+
+open HashFunctionImpl
+
+
+assume val createBuff: size:FStar.UInt32.t -> buffer:suint8_p{length buffer = size}
+assume val valueToBuff:#a :eqtype -> value: a -> suint8_p
+assume val intToBuff: value: FStar.UInt32 -> suint8_p 
+assume val bufferConcat : b1 : suint8_p -> b2: suint8_p -> b3:suint8_p{length b3 = length b1 + length b2}
+assume val lstToBuff: #a :eqtype -> value: list(skipList a) -> suint8_p
+
+val hashF: #a: eqtype ->  value: a -> levels: FStar.UInt32.t -> lst:list(skipList a) -> hash:suint8_p -> suint8_p
+let hashF #a value levels lst =
+	let tempbuff1 = createBuff size1 in 
+	let tempbuff2 = createBuff size2 in 
+	let tempbuff3 = createBuff size3 in 
+	let tempbuff4 = createBuff size4 in 
+	let tempbuff5 = createBuff size5 in 
+	valueToBuff value tempbuff1;
+	intToBuff levels tempbuff2; 
+	bufferConcat buff1 buff2 tempbuff3; 
+	lstToBuff lst tempbuff4;
+	bufferConcat buff3 buff4 tempbuff5
+	hashLocal tempbuff5 hash
